EvalCBV.v
@@ -40,8 +40,9 @@ Inductive econtext :=
 | ECpair2 (a : expr) (b : econtext) : IsValue a -> econtext
 | ECinl (_ : type) (_ : econtext)
 | ECinr (_ : type) (_ : econtext)
-| ECmatch_pair (target : econtext) (_ : open_expr [CEexpr; CEexpr])
-| ECmatch_sum (target : econtext) (a b : open_expr [CEexpr])
+| ECfst (_ : econtext)
+| ECsnd (_ : econtext)
+| ECmatch (target : econtext) (a b : open_expr [CEexpr])
 .
 
 Inductive plug : econtext -> expr -> expr -> Prop :=
@@ -58,8 +59,9 @@ Inductive plug : econtext -> expr -> expr -> Prop :=
 | Ppair2 E e b a h : plug E e b -> plug (ECpair2 a E h) e (Epair a b)
 | Pinl E e e' t : plug E e e' -> plug (ECinl t E) e (Einl t e')
 | Pinr E e e' t : plug E e e' -> plug (ECinr t E) e (Einr t e')
-| Pmatch_pair E e target k : plug E e target -> plug (ECmatch_pair E k) e (Ematch_pair target k)
-| Pmatch_sum E e target k1 k2 : plug E e target -> plug (ECmatch_sum E k1 k2) e (Ematch_sum target k1 k2)
+| Pfst E e e' : plug E e e' -> plug (ECfst E) e (Efst e')
+| Psnd E e e' : plug E e e' -> plug (ECsnd E) e (Esnd e')
+| Pmatch E e target k1 k2 : plug E e target -> plug (ECmatch E k1 k2) e (Ematch target k1 k2)
 .
 
 Inductive step : expr -> expr -> Prop :=
@@ -70,16 +72,20 @@ Inductive step : expr -> expr -> Prop :=
     step e1' e2'
 | STapp t body arg : IsValue arg -> step (Eapp (Eabs t body) arg) (subst arg body)
 | STlet v main : IsValue v -> step (Elet v main) (subst v main)
-| STmatch_pair t1 t2 v1 v2 k : 
+| STfst v1 v2 :
     IsValue v1 ->
     IsValue v2 ->
-    step (Ematch_pair (Epair $$ t1 $$ t2 $$ v1 $$ v2) k) (subst_list [v1; v2] k)
-| STmatch_inl t1 t2 v k1 k2 : 
+    step (Efst (Epair v1 v2)) v1
+| STsnd v1 v2 :
+    IsValue v1 ->
+    IsValue v2 ->
+    step (Esnd (Epair v1 v2)) v2
+| STmatch_inl t v k1 k2 : 
     IsValue v ->
-    step (Ematch_sum (Einl $$ t1 $$ t2 $$ v) k1 k2) (subst v k1)
-| STmatch_inr t1 t2 v k1 k2 : 
+    step (Ematch (Einl t v) k1 k2) (subst v k1)
+| STmatch_inr t v k1 k2 : 
     IsValue v ->
-    step (Ematch_sum (Einr $$ t1 $$ t2 $$ v) k1 k2) (subst v k2)
+    step (Ematch (Einr t v) k1 k2) (subst v k2)
 | STtapp body t : step (Etapp (Etabs body) t) (subst t body)
 | STunfold_fold v t1 : 
     IsValue v ->
